pulse/examples/steel/Queue.fst
@@ -10,7 +10,7 @@ let pure_upd_next
 assume
 val upd_next
   (#a: Type0) (#u: _) (#v: Ghost.erased (cell a)) (x:t a) (nxt:t a)
-     : SteelAtomic unit u (pts_to x v)
+     : SteelSelAtomic unit u (pts_to x v)
                             (fun _ -> pts_to x (pure_upd_next v nxt))
                             (requires (fun _ -> True))
                             (ensures (fun _ _ _ -> True))
@@ -19,30 +19,34 @@ let rec fragment
   (#a: Type0)
   (pstart: Ghost.erased (ref (cell a)))
   (l: Ghost.erased (list (ref (cell a) & cell a)))
-: Tot slprop
+: Tot vprop
   (decreases (Ghost.reveal l))
 =
   match Ghost.reveal l with
   | [] -> emp
   | (pa, a) :: q -> pts_to pa a `star` fragment a.next q `star` pure (Ghost.reveal pstart == pa)
 
-let slprop_extensionality (p q:slprop)
+(* AF: Does not hold for generic vprops, but holds for those in this module.
+   TODO: Fix proofs and remove axiom *)
+let slprop_extensionality (p q:vprop)
   : Lemma
     (requires p `equiv` q)
     (ensures p == q)
     [SMTPat (p `equiv` q)]
-=
-  slprop_extensionality p q
+= admit()
 
 inline_for_extraction noextract let canon () : FStar.Tactics.Tac unit =
-  (Steel.Memory.Tactics.canon ())
+  (FStar.Tactics.norm [delta_attr [`%__reduce__]]; canon' false (`true_p) (`true_p))
+
+let _: squash (forall p q. p `equiv` q <==> hp_of p `Steel.Memory.equiv` hp_of q) =
+  Classical.forall_intro_2 reveal_equiv
 
 let emp_equiv_pure
   (p: prop)
 : Lemma
   (requires p)
   (ensures (emp `equiv` pure p))
-=
+= reveal_emp ();
   Classical.forall_intro intro_emp;
   Classical.forall_intro (pure_interp p)
 
@@ -114,7 +118,7 @@ let queue_lc
   (hd tl: Ghost.erased (ref (cell a)))
   (l: Ghost.erased (list a))
   (lc: Ghost.erased (list (ref (cell a) & cell a)))
-: Tot slprop
+: Tot vprop
 = fragment hd lc `star` pure (queue_lc_prop tl l lc)
 
 let queue_l
@@ -126,21 +130,21 @@ let new_queue
   #a v
 =
   let c : cell a = {data = v; next = null} in
-  let pc : t a = alloc c in
+  let pc : t a = alloc_pt c in
   intro_pure (queue_lc_prop pc [v] [(pc, c)]);
   intro_pure (Ghost.reveal (Ghost.hide pc) == pc);
-  change_slprop ((pts_to pc c `star` emp `star` pure (Ghost.reveal (Ghost.hide pc) == pc)) `star` pure (queue_lc_prop pc [v] [(pc, c)])) (queue_lc pc pc [v] [(pc, c)]) (fun _ -> ());
+  rewrite_slprop ((pts_to pc c `star` emp `star` pure (Ghost.reveal (Ghost.hide pc) == pc)) `star` pure (queue_lc_prop pc [v] [(pc, c)])) (queue_lc pc pc [v] [(pc, c)]) (fun _ -> ());
   intro_exists (Ghost.hide [(pc, c)]) (queue_lc pc pc [v]);
   intro_exists (Ghost.hide [v]) (queue_l pc pc);
   return pc
 
 #push-options "--ide_id_info_off --print_implicits"
 
-let witness_h_exists_erased (#a:Type) (#opened_invariants:_) (#p: Ghost.erased a -> slprop) (_:unit)
-  : SteelGhostT (Ghost.erased a) opened_invariants
+let witness_h_exists_erased (#a:Type) (#opened_invariants:_) (#p: Ghost.erased a -> vprop) (_:unit)
+  : SteelSelGhostT (Ghost.erased a) opened_invariants
                 (h_exists p) (fun x -> p x)
 =
-  let w = witness_h_exists #(Ghost.erased a) #_ #p () in
+  let w = witness_exists #(Ghost.erased a) #_ #p () in
   Ghost.reveal w
 
 let snoc_inj (#a: Type) (hd1 hd2: list a) (tl1 tl2: a) : Lemma
@@ -166,16 +170,16 @@ let enqueue
 =
   let l : (Ghost.erased (list a)) = witness_h_exists_erased () in
   let lc0 : Ghost.erased (list (ref (cell a) & cell a)) = witness_h_exists_erased () in
-  change_slprop (queue_lc hd tl l lc0) (fragment hd lc0 `star` pure (queue_lc_prop tl l lc0)) (fun _ -> ());
+  rewrite_slprop (queue_lc hd tl l lc0) (fragment hd lc0 `star` pure (queue_lc_prop tl l lc0)) (fun _ -> ());
   elim_pure (queue_lc_prop tl l lc0);
   (* I don't have a pointer to the next field, so I need to manually change the next field of the last cell of the list *)
   let lc : (lc: Ghost.erased (list (ref (cell a) & cell a)) { Cons? (Ghost.reveal lc) }) = lc0 in
-  change_slprop (fragment hd lc0) (fragment hd lc) (fun _ -> ());
+  rewrite_slprop (fragment hd lc0) (fragment hd lc) (fun _ -> ());
   let lhd = Ghost.hide (unsnoc_hd (Ghost.reveal lc)) in
   let ltl = Ghost.hide (unsnoc_tl (Ghost.reveal lc)) in
   L.lemma_append_last lhd [Ghost.reveal ltl];
   next_last_correct hd lc;
-  change_slprop
+  rewrite_slprop
     (fragment hd lc)
     (fragment hd lhd `star` (pts_to tl (Ghost.hide (snd ltl)) `star` emp `star` pure (next_last hd lhd == fst ltl)))
     (fun _ -> fragment_append hd lhd [Ghost.reveal ltl]);
@@ -184,13 +188,13 @@ let enqueue
   let lc1 : (lc: Ghost.erased (list (ref (cell a) & cell a)) { Cons? (Ghost.reveal lc) }) = Ghost.hide (lhd `L.append` [(fst ltl, Ghost.reveal c1)]) in
   next_last_correct hd lc1;
   L.lemma_append_last lhd [(fst ltl, Ghost.reveal c1)];
-  change_slprop
+  rewrite_slprop
     (fragment hd lhd `star` (pts_to tl _  `star` emp `star` pure (next_last hd lhd == fst ltl)))
     (fragment hd lc1)
     (fun _ -> fragment_append hd lhd [(fst ltl, Ghost.reveal c1)]);
   intro_pure (Ghost.reveal (Ghost.hide last) == last);
   let lc2 = Ghost.hide (lc1 `L.append` [(last, Ghost.reveal v)]) in
-  change_slprop
+  rewrite_slprop
     (fragment hd lc1 `star` (pts_to last _ `star` emp `star` pure (Ghost.reveal (Ghost.hide last) == last)))
     (fragment hd lc2)
     (fun _ -> fragment_append hd lc1 [(last, Ghost.reveal v)]);
@@ -200,13 +204,13 @@ let enqueue
   L.map_append get_data lc1 [(last, Ghost.reveal v)];
   L.lemma_append_last lc1 [(last, Ghost.reveal v)];
   intro_pure (queue_lc_prop last l2 lc2);
-  change_slprop (fragment hd lc2 `star` pure (queue_lc_prop last l2 lc2)) (queue_lc hd last l2 lc2) (fun _ -> ());
+  rewrite_slprop (fragment hd lc2 `star` pure (queue_lc_prop last l2 lc2)) (queue_lc hd last l2 lc2) (fun _ -> ());
   intro_exists lc2 (queue_lc hd last l2);
   intro_exists l2 (queue_l hd last)
 
 assume
 val read_next (#a: _) (#u: _) (#v: _) (x:t a)
-    : SteelAtomic (t a) u (pts_to x v)
+    : SteelSelAtomic (t a) u (pts_to x v)
                             (fun _ -> pts_to x v)
                             (requires (fun _ -> True))
                             (ensures (fun _ res _ -> res == v.next))
@@ -216,20 +220,20 @@ let dequeue
 =
   let l : (Ghost.erased (list a)) = witness_h_exists_erased () in
   let lc0 : Ghost.erased (list (ref (cell a) & cell a)) = witness_h_exists_erased () in
-  change_slprop (queue_lc hd tl l lc0) (fragment hd lc0 `star` pure (queue_lc_prop tl l lc0)) (fun _ -> ());
+  rewrite_slprop (queue_lc hd tl l lc0) (fragment hd lc0 `star` pure (queue_lc_prop tl l lc0)) (fun _ -> ());
   elim_pure (queue_lc_prop tl l lc0);
   let l1 : (l1: Ghost.erased (list a) { Cons? l1 }) = Ghost.hide (Ghost.reveal l) in
   let l2 : Ghost.erased (list a) = Ghost.hide (L.tl l1) in
   let lc : (lc: Ghost.erased (list (ref (cell a) & cell a)) { Cons? (Ghost.reveal lc) }) = lc0 in
-  change_slprop (fragment hd lc0) (fragment hd lc) (fun _ -> ());
+  rewrite_slprop (fragment hd lc0) (fragment hd lc) (fun _ -> ());
   let lhd : Ghost.erased (ref (cell a) & cell a) = Ghost.hide (L.hd lc) in
   let ltl = Ghost.hide (L.tl lc) in
-  change_slprop
+  rewrite_slprop
     (fragment hd lc)
     (pts_to (fst lhd) (snd lhd) `star` fragment (snd lhd).next ltl `star` pure (Ghost.reveal hd == fst lhd))
     (fun _ -> ());
   elim_pure (Ghost.reveal hd == fst lhd);
-  change_slprop
+  rewrite_slprop
     (pts_to (fst lhd) (snd lhd))
     (pts_to hd (snd lhd))
     (fun _ -> ());
@@ -238,22 +242,22 @@ let dequeue
   then begin
     (* we need to repack everything back to the initial queue slprop *)
     intro_pure (Ghost.reveal hd == fst lhd);
-    change_slprop
+    rewrite_slprop
       (pts_to hd (snd lhd) `star` fragment (snd lhd).next ltl `star` pure (Ghost.reveal hd == fst lhd))
       (fragment hd lc0)
       (fun _ -> ());
     intro_pure (queue_lc_prop tl l lc0);
-    change_slprop (fragment hd lc0 `star` pure (queue_lc_prop tl l lc0)) (queue_lc hd tl l lc0) (fun _ -> ());
+    rewrite_slprop (fragment hd lc0 `star` pure (queue_lc_prop tl l lc0)) (queue_lc hd tl l lc0) (fun _ -> ());
     intro_exists lc0 (queue_lc hd tl l);
     intro_exists l (queue_l hd tl);
     return None
   end else begin
-    change_slprop
+    rewrite_slprop
       (fragment (snd lhd).next ltl)
       (fragment p ltl)
       (fun _ -> ());
     intro_pure (queue_lc_prop tl l2 ltl);
-    change_slprop
+    rewrite_slprop
       (fragment p ltl `star` pure (queue_lc_prop tl l2 ltl))
       (queue_lc p tl l2 ltl)
       (fun _ -> ());
